\begin{alignat*}{3}
G = \unknownVar{k_p} \dfrac{\unknownVar{Z_p(s)}}{\knownVar{R_p(s)}}
\qquad & M &= \knownVar{k_m \dfrac{Z_m(s)}{R_p(s)}}
\end{alignat*}
``We are happy with the plant poles $R_p(s)$''

\subsubsection*{Matching condition}
\paragraph{Problem}
\redtext{Zeroes cannot be changed by feedback}%
    \footnote{In feedback, poles can be moved, but 
    zeroes have to be cancelled out}

\paragraph{Solution}
Design an \greentext{adaptive feedforward controller}
to cancel plant zeroes and introudce model zeroes

\begin{conclusion}{darkgreen}
\begin{alignat*}{3}
C^*(s) \overset{!}{=} \dfrac{k_m}{k_p} \cdot \dfrac{Z_m(s)}{Z_p(s)}
\end{alignat*}
Note%
\footnote{? ``unparametrised, doesn't lead to error dynamics ?}
\end{conclusion}

\begin{figure}[H]
    \centering
    \tikzsetnextfilename{ofac-zp-ff}
    \input{./img/ofac-zp-ff.tex}
\end{figure}

\begin{alignat*}{3}
C^*(s) G(s) \overset{!}{=} M(s)
\end{alignat*}

This is a structure that we know produces a ``linear in the
parameters error dynamics''.

\begin{figure}[H]
    \centering
    \tikzsetnextfilename{ofac-zp-filter}
    \input{./img/ofac-zp-filter.tex}
\end{figure}

\begin{alignat*}{3}
\theta_1(t), \phi_1(t) &\in \R^{n-1}\\
k(t), l &\in \R^1
\end{alignat*}

The filter $F(s)$ can be described by
\begin{alignat*}{3}
\dot{ \phi_1}(t) &= \Lambda \phi_1(t) + lu(t)
\end{alignat*}

where $\Lambda$ is a $(n - 1) \times (n - 1)$
asymptotically stable matrix.
$\left[ \Lambda, l \right]$ is controllable
$\corresponds \phi_i$ is linear independent.

\paragraph{State controllability}
implies that any end state $x_f$ is reachable
given an initial state $x_0$.
However, this \redtext{doesn't mean that
the state remains at $x_f$}.
A prerequisite for state controllability is
that the states must be \greentext{linear independent},
i.e. enables free movement anywhere.\\

$ \phi_i$ linear independent $\Rightarrow \theta_i$
amount needed. If not:
\begin{itemize}
\item Reduced number of $\theta$ elements
\item Reduced information
\end{itemize}

The input $u$ is
\begin{alignat*}{3}
u(t) &= \theta_1^T(t) \phi_1(t) + k(t) r(t)
\end{alignat*}

Assume constants for $ \theta_1 = \theta_{1c}$
and $k = k_c$. Pick some $\left[ \Lambda, l \right]$ 
with $\Lambda$ stable,
\begin{alignat*}{3}
F &= \left( sI - \Lambda \right)^{-1} l
\end{alignat*}

The feedback loop is
\begin{alignat*}{3}
\theta_{1c}^T \left( sI - \Lambda \right)^{-1} l
    \corresponds \dfrac{p(s)}{\lambda(s)}
\end{alignat*}

where $\lambda(s)$ is the characteristic polynomial
of $\left( sI - \lambda \right)$ (chosen beforehand).

(with constant assumption)
\begin{alignat*}{3}
\dfrac{u}{r} = C(s) = k_c \dfrac{\lambda(s)}{\lambda(s) - p(s)}
\end{alignat*}

\paragraph{Discussion}
We pick $\Lambda, \lambda(s)$ 
\begin{itemize}
\item The adaptive parameters $\theta_{1c}$ decide on $p(s)$
\item From $C^*$ we know that we should pick
    $\Lambda \rightsquigarrow \lambda(s) = Z_m(s)$\\
    (possible, since order of $Z_m(s)$ is $n-1 $)
\item Comparing $C^*$ and $C$, we find
\begin{alignat*}{3}
Z_p(s) &\overset{!}{=} \lambda(s) - p^*(s)\\
\Leftrightarrow p(s) &= \lambda(s) - Z_p(s)\\
    &= Z_m(s) Z_p(s)
\end{alignat*}
\end{itemize}

Since $Z_m(s), Z_p(s)$ are monic of order $n-1$,
$Z_m(s), Z_p(s)$ is of order $n-2$.
Also,  $p$ is of order $n-2 \Rightarrow$
it is possible tose $k_c$ and $\theta_{1c}$,
such that $C(s) = C^*(s)$.\\

\begin{conclusion}{darkgreen}
$\Rightarrow$ \textbf{Matching condition holds}, i.e.
\begin{alignat*}{3}
\exists ~ \theta &\corresponds \left[ k^*, \theta^{*T} \right]^T\\
\txt{s.t.} \quad  y_p &= y_m \quad \txt{for } t \rightarrow \infty
\end{alignat*}
\end{conclusion}

\subsubsection*{Error dynamics}
\begin{alignat*}{3}
\tilde{\theta} &= \matr{ \tilde{\theta}_1 \\ \tilde{k}}
    \in \R^n
\end{alignat*}

\begin{alignat*}{3}
&\txt{Plant P} \quad  &
    \dot{x}_p(t) &= a_p x_p(t) + b_p u\\
    && y_p(t) &= c_p^T x_p(t)\\
~\\
&\txt{Controller}  \quad &
    \dot{ \phi_1}(t) &= \Lambda \phi_1 + lu\\
    && u &= \theta_1^T \phi_1 + kr
\end{alignat*}

Note: adaptive law is missing here.\\
Substituting $u$ in $P $:
\begin{alignat*}{3}
\dot{x}_p(t)
    &= a_p x_p(t) + b_p \theta_1^T \phi + b_p k_r\\
    &= a_p x_p(t) + b_p \theta_1^{*T} \phi_1 + b_p k^* r\\
    & \quad + b_p \matr{ \tilde{\theta}_1^T & \tilde{k}}
        \matr{ \phi \\ r}\\
\dot{\phi} &= \Lambda \phi_1 + l \theta_1^{*T} \phi_1
    + lk^*r + l \matr{ \tilde{\theta}_1^T & \tilde{k}} \matr{ \phi_1 \\ r}
\end{alignat*}

